Compile.v
@@ -5,26 +5,34 @@ From Vyper Require Import Config Calldag.
 From Vyper.L10 Require AST Callset Descend Interpret.
 From Vyper.From10To20 Require FunCtx Call.
 From Vyper.From20To30 Require FunCtx Call.
+From Vyper.CheckArith Require Builtins Translate Call.
 From Vyper Require Import ConstFold L10.Base.
 
 (** This is the verified part of the compiler.
     This function translates a L10 calldag into a L30 calldag (or an error).
  *)
-Definition translate_10_to_30 {C: VyperConfig} (calldag10: L10.Descend.calldag)
+Definition translate_10_to_30 {C: VyperConfig} (B: CheckArith.Builtins.builtin_names_config)
+                              (calldag10: L10.Descend.calldag)
 : string + L30.Descend.calldag
 := let calldag20 := From10To20.FunCtx.translate_calldag calldag10 (* no errors possible *) in
    match const_fold_calldag calldag20 with
    | inl err => inl err
-   | inr calldag20' => From20To30.FunCtx.translate_calldag calldag20'
+   | inr calldag20' =>
+      match From20To30.FunCtx.translate_calldag calldag20' with
+      | inl err => inl err
+      | inr calldag30 => inr (CheckArith.Translate.translate_calldag B calldag30)
+      end
    end.
 
 (** This is the theorem verifying that the compiler works as intended.
  *)
 Theorem translate_10_to_30_ok {C: VyperConfig}
+                              (B: CheckArith.Builtins.builtin_names_config)
                               (calldag10: L10.Descend.calldag)
                               (calldag30: L30.Descend.calldag)
-                              (ok: translate_10_to_30 calldag10 = inr calldag30)
+                              (ok: translate_10_to_30 B calldag10 = inr calldag30)
                               (builtins: string -> option builtin)
+                              (BuiltinsOk: Builtins.BuiltinsSupportUInt256 B builtins)
                               (fun_name: string)
                               (world: world_state)
                               (arg_values: list uint256):
@@ -45,7 +53,14 @@ rewrite<- (const_fold_ok _ Heqcalldag20').
 clear Heqcalldag20'.
 
 (* 20 -> 30 *)
-apply From20To30.Call.translate_ok. exact ok.
+remember (FunCtx.translate_calldag calldag20') as calldag30_ops. symmetry in Heqcalldag30_ops.
+destruct calldag30_ops as [|calldag30_ops]. { discriminate. }
+rewrite<- (From20To30.Call.translate_ok builtins _ _ Heqcalldag30_ops).
+clear Heqcalldag30_ops.
+
+(* check arith *)
+inversion ok. subst calldag30.
+apply (CheckArith.Call.translate_ok builtins BuiltinsOk).
 Qed.
 
 (** This function takes the parser output, which is a list of L10 declarations,
@@ -53,11 +68,13 @@ Qed.
 
     Here [make_calldag] converts the output of the parser to the input to the verified compiler.
  *)
-Definition compile_to_L30 {C: VyperConfig} (parsed_src: list L10.AST.decl)
+Definition compile_to_L30 {C: VyperConfig}
+                          (B: CheckArith.Builtins.builtin_names_config)
+                          (parsed_src: list L10.AST.decl)
 : string + L30.Descend.calldag
 := match make_calldag L10.AST.decl_name L10.Callset.decl_callset parsed_src with
    | inl err => inl err
-   | inr cd => translate_10_to_30 cd
+   | inr cd => translate_10_to_30 B cd
    end.
 
 Definition calldag_to_string {C: VyperConfig} (cd: L30.Descend.calldag)
@@ -67,9 +84,11 @@ Definition calldag_to_string {C: VyperConfig} (cd: L30.Descend.calldag)
                               (Map.items (cd_decls cd))))%string.
 
 (** This is the compiler without parser. *)
-Definition compile {C: VyperConfig} (parsed_src: list L10.AST.decl)
+Definition compile {C: VyperConfig}
+                   (B: CheckArith.Builtins.builtin_names_config)
+                   (parsed_src: list L10.AST.decl)
 : string + string
-:= match compile_to_L30 parsed_src with
+:= match compile_to_L30 B parsed_src with
    | inl err => inl err
    | inr cd => inr (calldag_to_string cd)
    end.
