CheckArith/Call.v
@@ -1,0 +1,158 @@
+From Coq Require Import Arith NArith ZArith Lia String.
+
+From Vyper Require Import Logic2.
+From Vyper Require Import Config L10.Base Calldag.
+From Vyper Require OpenArray.
+From Vyper Require Import UInt256.
+From Vyper.L30 Require Import AST Stmt Callset VarCap Interpret.
+From Vyper.CheckArith Require Import CheckedArith Translate Builtins Stmt.
+
+Lemma translate_call_ok {C: VyperConfig}
+                        {bigger_call_depth_bound smaller_call_depth_bound: nat}
+                        (Ebound: bigger_call_depth_bound = S smaller_call_depth_bound)
+                        (builtins: string -> option L10.Base.builtin)
+                        {B: builtin_names_config}
+                        (BuiltinsOk: BuiltinsSupportUInt256 B builtins)
+                        {cd: L30.Descend.calldag}
+                        (fc: fun_ctx cd bigger_call_depth_bound)
+                        (world: world_state)
+                        (arg_values: list uint256):
+  interpret_call builtins (translate_fun_ctx B fc) world arg_values
+   =
+  interpret_call builtins fc world arg_values.
+Proof.
+revert world arg_values smaller_call_depth_bound Ebound. induction bigger_call_depth_bound.
+{ exfalso. exact (Nat.nlt_0_r _ (proj1 (Nat.ltb_lt _ _) (fun_bound_ok fc))). }
+intros. cbn.
+assert(F: cached_mapped_decl (translate_decl B) (Translate.translate_calldag_helper B cd) cd fc
+           =
+          translate_decl B (fun_decl fc)).
+{
+  clear IHbigger_call_depth_bound.
+  unfold cached_mapped_decl.
+  remember (Calldag.calldag_map_fun_ctx_fun_decl_helper _ _ cd fc) as foo.
+  clear Heqfoo.
+  remember (cd_declmap (calldag_map (translate_decl B) (Translate.translate_calldag_helper B cd) cd)
+    (fun_name fc)) as d.
+  destruct d. 2:{ contradiction. }
+  subst.
+  assert (Q := calldag_map_declmap (translate_decl B) (Translate.translate_calldag_helper B cd) cd (fun_name fc)).
+  destruct (cd_declmap (calldag_map (translate_decl B) (Translate.translate_calldag_helper B cd) cd) (fun_name fc)) as [d'|]. 2:discriminate.
+  inversion Heqd. subst d'. clear Heqd.
+  remember (cd_declmap cd (fun_name fc)) as x.
+  destruct x as [x|]. 2:discriminate.
+  inversion Q. f_equal.
+  assert (D := fun_decl_ok fc).
+  rewrite D in *. inversion Heqx.
+  trivial.
+}
+intros.
+cbn.
+remember (fun name arity body
+              (E: cached_mapped_decl (translate_decl B) (Translate.translate_calldag_helper B cd) cd fc =
+                      FunDecl name arity body) =>
+      if Datatypes.length arg_values =? N.to_nat arity
+          then
+           let
+           '(world', _, result) :=
+            interpret_stmt eq_refl (translate_fun_ctx B fc) (interpret_call builtins) builtins world
+              (OpenArray.from_list arg_values) body (Interpret.interpret_call_helper E) in
+            (world',
+            match result with
+            | StmtSuccess => ExprSuccess zero256
+            | StmtAbort a => ExprAbort a
+            | StmtReturnFromFunction x => ExprSuccess x
+            end)
+          else
+           (world,
+           expr_error
+             (if match N.to_nat arity with
+                 | 0 => false
+                 | S m' => Datatypes.length arg_values <=? m'
+                 end
+              then "function called with too few arguments"%string
+              else "function called with too many arguments"%string))
+) as branch_l.
+remember (fun name arity body
+              (E : fun_decl fc = FunDecl name arity body) =>
+  if Datatypes.length arg_values =? N.to_nat arity
+    then
+     let
+     '(world', _, result) :=
+      interpret_stmt eq_refl fc (interpret_call builtins) builtins world
+        (OpenArray.from_list arg_values) body (Interpret.interpret_call_helper E) in
+      (world',
+      match result with
+      | StmtSuccess => ExprSuccess zero256
+      | StmtAbort a => ExprAbort a
+      | StmtReturnFromFunction x => ExprSuccess x
+      end)
+    else
+     (world,
+     expr_error
+       (if match N.to_nat arity with
+           | 0 => false
+           | S m' => Datatypes.length arg_values <=? m'
+           end
+        then "function called with too few arguments"%string
+        else "function called with too many arguments"%string))) as branch_r.
+enough (Ok: forall name arity body_l body_r E_l E_r,
+             branch_l name arity body_l E_l
+              =
+             branch_r name arity body_r E_r).
+{
+  clear Heqbranch_l Heqbranch_r.
+  destruct (fun_decl fc); cbn in F; destruct cached_mapped_decl; try easy.
+  inversion F; subst.
+  apply Ok.
+}
+intros. subst.
+destruct (Datatypes.length arg_values =? N.to_nat arity). 2:easy.
+
+rewrite E_l in F. rewrite E_r in F.
+cbn in F. inversion F; subst body_l; clear F.
+rename body_r into body.
+
+assert (DoCallOk: forall (fc : fun_ctx cd bigger_call_depth_bound)
+                              (world : world_state) (arg_values : list uint256),
+                            interpret_call builtins (translate_fun_ctx B fc) world arg_values =
+                            interpret_call builtins fc world arg_values).
+{
+  intros.
+  destruct bigger_call_depth_bound as [|n]. { easy. }
+  now apply IHbigger_call_depth_bound with (smaller_call_depth_bound := n).
+}
+assert (T := let _ := memory_impl in
+             translate_stmt_ok eq_refl builtins B (var_cap_stmt body) BuiltinsOk
+             fc DoCallOk body
+             (Interpret.interpret_call_helper E_l)
+             (Interpret.interpret_call_helper E_r)
+             world
+             (OpenArray.from_list arg_values)
+             (OpenArray.from_list arg_values)
+             (N.le_refl _)
+             (fun _ _ => eq_refl)).
+cbn in T.
+destruct interpret_stmt as ((w', m'), result'); destruct interpret_stmt as ((w, m), result).
+destruct T as (Rresult, (Rw, _)). subst. trivial.
+Qed.
+
+Theorem translate_ok {C: VyperConfig}
+                     (builtins: string -> option L10.Base.builtin)
+                     {B: builtin_names_config}
+                     (BuiltinsOk: BuiltinsSupportUInt256 B builtins)
+                     (cd: L30.Descend.calldag)
+                     (fun_name: string)
+                     (world: world_state)
+                     (arg_values: list uint256):
+  interpret builtins (translate_calldag B cd) fun_name world arg_values
+   =
+  interpret builtins cd fun_name world arg_values.
+Proof.
+unfold interpret.
+unfold translate_calldag.
+rewrite (make_fun_ctx_and_bound_map (translate_decl B) _).
+destruct (make_fun_ctx_and_bound cd fun_name) as [(bound, fc)|]; cbn. 2:{ trivial. }
+destruct bound. { easy. }
+apply (translate_call_ok eq_refl builtins BuiltinsOk fc world arg_values).
+Qed.
